Set_Graphs/Graph_Algorithms/Array_Map_Iterator.thy
@@ -1,0 +1,203 @@
+theory Array_Map_Iterator
+  imports Separation_Logic_Imperative_HOL_Partial.Array_Map_Impl
+begin
+
+subsection \<open>Iterators\<close>
+
+subsubsection \<open>Definitions\<close>
+type_synonym 'v iam_it = "(nat \<times> 'v array_map)"
+
+partial_function (heap) iam_it_adjust :: "('v::heap) iam_it \<Rightarrow> ('v iam_it) Heap" where
+ "iam_it_adjust it =
+  (case it of (i, A) \<Rightarrow> 
+    do{l \<leftarrow> Array.len A;
+       if i \<ge> l then return (l, A)
+       else do {x \<leftarrow> Array.nth A i;
+               case x of None \<Rightarrow> iam_it_adjust (Suc i, A)
+               | Some _ \<Rightarrow> return (i, A) }})"
+
+
+definition iam_it_init 
+  :: "('v::heap) array_map \<Rightarrow> ('v iam_it) Heap"
+  where 
+  "iam_it_init A \<equiv> do {
+   let it = (0, A);
+   iam_it_adjust it}"
+
+definition iam_it_has_next 
+  :: "('v::heap) iam_it \<Rightarrow> bool Heap"
+  where "iam_it_has_next it 
+  \<equiv> case it of (i, A) \<Rightarrow>
+     do {l \<leftarrow> Array.len A;
+         return (i < l)}"
+
+definition iam_it_next::"('v::heap) iam_it \<Rightarrow> ((nat \<times> 'v) \<times> 'v iam_it) Heap"
+  where "iam_it_next it = 
+  (case it of (i, A) \<Rightarrow>
+    do {x \<leftarrow> Array.nth A i;
+        it' \<leftarrow> iam_it_adjust (Suc i, A);
+        return ((i, the x), it')})"
+
+definition "iam_is_it m A m' = (\<lambda> (i, A').
+      (\<exists>\<^sub>Al. A\<mapsto>\<^sub>al * \<up>(m=iam_of_list l \<and> A = A' \<and> i \<le> length l \<and> (i < length l \<longrightarrow> l ! i \<noteq> None)
+            \<and> m' = (\<lambda> j. if j \<ge> i then iam_of_list (drop i l) (j - i) else None))))"
+
+definition "iam_is_it' m A m' = (\<lambda> (i, A').
+      (\<exists>\<^sub>Al. A\<mapsto>\<^sub>al * \<up>(m=iam_of_list l \<and> A = A' \<and> i \<le> length l
+            \<and> m' = (\<lambda> j. if j \<ge> i then iam_of_list (drop i l) (j - i) else None))))"
+
+lemma is_am_implies_iam_is_it':"is_iam m A \<Longrightarrow>\<^sub>A iam_is_it' m A m (0, A)"
+  by(sep_auto simp: is_iam_def iam_is_it'_def)
+
+lemma iam_it_adjust_rule:
+  "<iam_is_it' m A m' (i, A')> iam_it_adjust (i, A') <iam_is_it m A m'>"
+proof(induction arbitrary: i rule: iam_it_adjust.fixp_induct, goal_cases)
+  case 1
+  then show ?case 
+    by simp
+next
+  case 2
+  then show ?case 
+    by simp
+next
+  case (3 f i)
+  show ?case
+    unfolding iam_is_it'_def
+    unfolding prod.case
+    apply(rule ht_exEI)
+    subgoal for l
+      apply(rule ht_bind[where R = 
+    "\<lambda> r. A \<mapsto>\<^sub>a l * \<up> (m = iam_of_list l \<and> A = A' \<and> i \<le> length l 
+              \<and> m' = (\<lambda>j. if i \<le> j then iam_of_list (drop i l) (j - i) else None) \<and> r = length l)"])
+      subgoal
+        by sep_auto
+      apply(clarsimp split!: if_split)
+      subgoal for len
+        by(sep_auto  simp: iam_is_it_def)
+      subgoal for len
+        apply(rule ht_bind[where R = "\<lambda> r. 
+             A \<mapsto>\<^sub>a l *
+     \<up> (m = iam_of_list l \<and> A = A' \<and> i \<le> length l \<and> m' = (\<lambda>j. if i \<le> j then iam_of_list (drop i l) (j - i) else None) 
+            \<and> len = length l \<and> r = l ! i \<and> i < length l)"])
+        subgoal
+          by sep_auto
+        subgoal for x
+          apply(cases x)
+          subgoal
+            apply simp
+            apply(rule ht_cons_pre[OF _ 3])
+            apply(sep_auto simp: iam_is_it'_def)
+            apply(rule ent_ex_postI[of _ _ l])
+            apply sep_auto 
+            apply(rule ext)
+            by (auto simp add: iam_of_list_def)
+          subgoal for xx
+            apply simp
+            apply (sep_auto simp: iam_is_it_def)
+            apply(rule mod_exI[of _ l])
+            apply (sep_auto simp:  mod_pure_star_dist)
+            using domIff by fastforce
+          done
+        done
+      done
+    done
+qed
+
+lemma iam_it_init_rule:
+  "<is_iam m A> iam_it_init A <iam_is_it m A m>"
+  unfolding iam_it_init_def
+  unfolding Let_def
+  apply(rule ht_cons_pre)
+  apply(rule  is_am_implies_iam_is_it')
+  by(rule iam_it_adjust_rule)
+
+lemma assn_ex_impl_same_witness: "(\<And> x. P x \<Longrightarrow>\<^sub>A Q x) \<Longrightarrow> \<exists>\<^sub>A x. P x \<Longrightarrow>\<^sub>A \<exists>\<^sub>A x. Q x"
+  apply(rule ent_ex_preI)
+  apply(rule ent_ex_postI)
+  by auto
+
+lemma iam_it_next_rule:
+  assumes "m' \<noteq> (\<lambda>x. None)"
+  shows "<iam_is_it m A m' it> iam_it_next it
+    <\<lambda>((k, v), it'). iam_is_it m A (m' |` (- {k})) it' * \<up> (m' k = Some v)>"
+  unfolding iam_it_next_def
+  apply(cases it)
+  subgoal for i A'
+    apply simp
+    apply(rule ht_bind[where R = "\<lambda> r. iam_is_it m A m' (i, A')* \<up> (r = m' i \<and> (\<exists> rr. r = Some rr))"])
+    subgoal
+      apply(sep_auto simp: iam_is_it_def)
+      subgoal for l a b y
+        apply(rule mod_exI[of _ l])
+        by (sep_auto simp: iam_of_list_def)
+      done
+    subgoal for xx
+      apply(rule ht_cons_pre[where P' = "iam_is_it' m A (m' |` (- {i})) (Suc i, A')*
+                    \<up> (xx = m' i \<and> (\<exists>rr. xx = Some rr))"])
+      subgoal
+        apply (sep_auto simp: iam_is_it'_def iam_is_it_def)
+        apply(rule assn_ex_impl_same_witness)
+        subgoal for l
+          using assms
+          apply (sep_auto simp: iam_of_list_def)
+          subgoal for a b rr y
+            apply(rule ext)
+            subgoal for j
+              apply(cases "Suc i \<le> j")
+              subgoal
+                by(auto simp add: iam_of_list_def)
+              subgoal 
+                by(cases "i \<le> j") auto
+              done
+            done
+          done
+        done
+      using iam_it_adjust_rule[of m A "m' |` (- {i})" "Suc i" A']
+      by sep_auto
+    done
+  done
+
+lemma iam_it_has_next_rule:
+  "<iam_is_it m p m' it> iam_it_has_next it <\<lambda>r. iam_is_it m p m' it * \<up> (r = (m' \<noteq> (\<lambda>x. None)))>"
+  unfolding iam_it_has_next_def
+  apply(cases it)
+  apply (sep_auto simp: iam_is_it_def)
+  subgoal for l a b
+    by (sep_auto intro: mod_exI[of _ l] simp: mod_pure_star_dist iam_of_list_def)
+  subgoal for i l a b y
+    apply(rule mod_exI[of _ l])
+    apply (sep_auto simp: mod_pure_star_dist iam_of_list_def)
+    by (metis (no_types, lifting) Cons_nth_drop_Suc diff_diff_cancel drop_all iam_lookup_abs1 le_eq_less_or_eq
+        length_drop list.size(3) nth_Cons_0 option.distinct(1) zero_less_diff)
+  done
+
+lemma iam_it_finish':
+  "iam_is_it m p m' it \<Longrightarrow>\<^sub>A is_iam m p"
+  by(cases it)
+    (sep_auto simp: iam_is_it_def is_iam_def)
+
+lemma iam_it_finish:
+  "iam_is_it m p m' it \<Longrightarrow>\<^sub>A is_iam m p * true"
+  by(cases it)
+    (sep_auto simp: iam_is_it_def is_iam_def)
+
+interpretation iam: imp_map_iterate is_iam iam_is_it iam_it_init iam_it_has_next iam_it_next
+proof( unfold_locales, goal_cases)
+  case (1 s p)
+  then show ?case 
+    using iam_it_init_rule by auto
+next
+  case (2 m' m A it)
+  then show ?case 
+    using iam_it_next_rule[of m' m A it] by simp
+  next
+  case (3 m p m' it)
+  then show ?case
+    using iam_it_has_next_rule[of m p m' it] by simp
+next
+  case (4 m p m' it)
+  then show ?case 
+    using  iam_it_finish[of m p m' it] by simp
+qed
+
+end
